Prove adequacy for `stateH`.

src/state.v
@@ -4,7 +4,10 @@ From iris.base_logic.lib Require Import ghost_var.
 From iris.base_logic.lib Require Export fancy_updates.
 From iris.itree Require Import handler.
 From iris.itree Require Import wpi.
+From iris.itree Require Import itree.
 From ITree Require Import ITree.
+From Paco Require Import paco.
+From Paco Require Import paco3.
 
 Class stateHPreG (Σ : gFunctors) (S : Type) := StateHPreG {
   stateH_pre_ghost_varG :> ghost_varG Σ S;
@@ -87,3 +90,125 @@ Section wp_state.
     iNext. rewrite -wpi_clear_mask. iMod "Hfupd". by iMod "Hwp".
   Qed.
 End wp_state.
+
+Section stateH_adequacy.
+  Context {S : Type} `{!stateHGS Σ S} {E : Type → Type} `{!invGS_gen HasNoLc Σ}.
+  Context `{!stateInterp Σ S}.
+  Context {H : iHandler Σ E} `{stateE S -< E} `{inH Σ (stateE S) E (stateH S) H}.
+  Context {R : Type}.
+  (** This sequentiality assumption is used for the [ForwardVis] case in the adequacy
+  proof below. *)
+  Context `{!Sequential H}.
+
+  (** The evaluation relation, prior to taking the fixpoint. This relation relates
+  an [itree (stateE S +' E) R] to its evaluated [itree E (S * R)] where the
+  final state is put in the first component of its return value. *)
+  Variant evalF
+    (eval : S → itree (stateE S +' E) R → itree E (S * R) → Prop)
+    : S
+    → itree' (stateE S +' E) R
+    → itree' E (S * R)
+    → Prop :=
+  (** Forwarding what doesn't affect the state. *)
+  | ForwardRet s r :
+    evalF eval s (RetF r) (RetF (s, r))
+  | ForwardTau s t t' :
+    eval s t t' →
+    evalF eval s (TauF t) (TauF t')
+  | ForwardVis s A e k k' :
+    (∀ a : A, eval s (k a) (k' a)) →
+    evalF eval s (VisF (inr1 e) k) (VisF e k')
+  (** Setting the state from [s] to [s']. *)
+  | SetState s s' k t :
+    eval s' (k tt) t →
+    evalF eval s (VisF (inl1 (ESetState s')) k) (TauF t)
+  (** Getting the state [s]. *)
+  | GetState s k t :
+    eval s (k s) t →
+    evalF eval s (VisF (inl1 EGetState) k) (TauF t).
+  Hint Constructors evalF : iris_itree.
+  Definition eval_
+    (eval : S → itree (stateE S +' E) R → itree E (S * R) → Prop)
+    : S
+    → itree (stateE S +' E) R
+    → itree E (S * R)
+    → Prop :=
+    λ s t t', evalF eval s (observe t) (observe t').
+
+  Lemma evalF_mono eval eval' s t t' :
+    eval <3= eval' →
+    evalF eval  s t t' →
+    evalF eval' s t t'.
+  Proof.
+    intros Hleq HevalF. destruct HevalF; eauto with iris_itree.
+  Qed.
+  Lemma eval__mono :
+    monotone3 eval_.
+  Proof.
+    rewrite /monotone3 /eval_. intros. by eapply evalF_mono; last done.
+  Qed.
+  Hint Resolve eval__mono : paco.
+
+  (** The evaluation relation. See comment above. *)
+  Definition eval :
+    S → itree (stateE S +' E) R → itree E (S * R) → Prop :=
+    paco3 eval_ bot3.
+
+  (** A technical version of adequacy, amenable to induction. See corollary below for a
+  more meaningful statement. *)
+  Theorem wpi_state' s t t' M Φ :
+    eval s t t' →
+    state_interp s -∗
+    WPi t @ stateH S ⊕ H; ∅ {{ v, |={∅, M}=> Φ v }} -∗
+    WPi t' @ H; ∅ {{ x, |={∅, M}=> let (s, v) := x in state_interp s ∗ Φ v }}.
+  Proof.
+    iIntros "%Heval Hstate Hwp".
+    iLöb as "IH" forall (t t' s Heval M Φ). punfold Heval.
+    inversion Heval as
+      [s_ r Hs Ht Ht'
+      |s_ t_ t_' Heval' Hs Ht Ht'
+      |s_ A e k k' Heval' Hs Ht Ht'
+      |s_ s_' k t_ Heval' Hs Ht Ht'
+      |s_ k t_ Heval' Hs Ht Ht'
+      ].
+    - (* ForwardRet s_ r *)
+      destruct Hs. apply ret_observe_eqit in Ht as <-. apply ret_observe_eqit in Ht' as <-.
+      rewrite -!wpi_ret'. iMod "Hwp". iModIntro. iMod "Hwp". iModIntro. iFrame.
+    - (* FowardTau s_ t_ t_' *)
+      destruct Hs. apply tau_observe_eqit in Ht as <-. apply tau_observe_eqit in Ht' as <-.
+      rewrite -!wpi_tau'. iMod "Hwp". iModIntro. iNext. iEval (rewrite wpi_update_post).
+      pclearbot. iApply ("IH" with "[//] Hstate"). rewrite wpi_update_post //.
+    - (* FowardVis s_ A e k k' *)
+      destruct Hs. apply vis_observe_eqit in Ht as <-. apply vis_observe_eqit in Ht' as <-.
+      rewrite -!wpi_vis'. iMod "Hwp". iModIntro.
+      iApply is_seq. iApply (ihandler_mono with "[Hstate] [] Hwp").
+      * iIntros (a) "Hwp". iNext. pclearbot. iEval (rewrite wpi_update_post).
+        iApply ("IH" with "[] Hstate").
+        + iPureIntro. apply Heval'.
+        + by iApply wpi_update_post.
+      * iModIntro. by iIntros (a) "Hwp".
+    - (* SetState s_ s_' k t_ *)
+      destruct Hs. apply vis_observe_eqit in Ht as <-. apply tau_observe_eqit in Ht' as <-.
+      rewrite -wpi_vis'. iMod "Hwp". simpl. iMod ("Hwp" $! s_ with "Hstate") as "[Hstate Hwp]".
+      iApply wpi_tau. iNext. pclearbot. iApply ("IH" with "[//] Hstate").
+      by iApply wpi_update_post.
+    - (* GetState s_ k t_ *)
+      destruct Hs. apply vis_observe_eqit in Ht as <-. apply tau_observe_eqit in Ht' as <-.
+      rewrite -wpi_vis'. iMod "Hwp". simpl. iDestruct ("Hwp" $! s_ with "Hstate") as "[Hstate Hwp]".
+      iApply wpi_tau. iNext. pclearbot. iApply ("IH" with "[//] Hstate").
+      by iApply wpi_update_post.
+  Qed.
+
+  (** Adequacy for [stateH S ⊕ H]. This says that if you can prove the
+  weakest precondition an [itree (stateE S +' E) R] then you get the weakest
+  precondition its evaluated [itree E (S * R)]. *)
+  Theorem wpi_state s t t' M Φ :
+    eval s t t' →
+    state_interp s -∗
+    WPi t @ stateH S ⊕ H; M {{ v, Φ v }} -∗
+    WPi t' @ H; M {{ x, let (s, v) := x in state_interp s ∗ Φ v }}.
+  Proof.
+    iIntros (Heval) "Hstate Hwp". rewrite -wpi_clear_mask. iEval (rewrite -wpi_clear_mask).
+    by iApply (wpi_state' with "Hstate").
+  Qed.
+End stateH_adequacy.
